Wrote up byte code

07ByteCode/ByteCode.thy
@@ -2,64 +2,84 @@ theory ByteCode
   imports "../00Utils/Environment" "../00Utils/Iteration"
 begin
 
-datatype byte_code = 
-  BLookup nat
-  | BPushCon nat
-  | BPushLam nat
-  | BApply
-  | BReturn
-  | BJump
+section \<open>Byte Code\<close>
 
-datatype bclosure = 
-  BConst nat
-  | BLam "bclosure list" nat
+text \<open>the last phase compiled to a tree-structured sort of code; but of course real code is not 
+tree-structured but linear. We therefore define a new sort of code, similar to tree-code but with 
+code-pointers everywhere we previously had recursive codeblocks. (We call it "bytecode" for a 
+memorable name and because it could easily be made into such, but we will never actually define a 
+representation ourselves.)\<close>
 
-datatype byte_code_state = 
-  BS "bclosure list" "(bclosure list \<times> nat) list"
+datatype code\<^sub>b = 
+  Lookup\<^sub>b nat
+  | PushCon\<^sub>b nat
+  | PushLam\<^sub>b nat
+  | Apply\<^sub>b
+  | Return\<^sub>b
+  | Jump\<^sub>b
 
-inductive evalb :: "byte_code list \<Rightarrow> byte_code_state \<Rightarrow> byte_code_state \<Rightarrow> bool" 
+datatype closure\<^sub>b = 
+  Const\<^sub>b nat
+  | Lam\<^sub>b "closure\<^sub>b list" nat
+
+datatype state\<^sub>b = 
+  S\<^sub>b "closure\<^sub>b list" "(closure\<^sub>b list \<times> nat) list"
+
+text \<open>The evaluation relation is rather similar to our previous one, except with code-pointers into
+our main bytecode block instead of storing the code in the stack and closures directly. The relation
+is now a three-place one, however: the bytecode is separate from the states. We could put it into 
+the state directly, but that would be misleading: the state is for data that changes at runtime, 
+like the various stacks, but the bytecode never changes. In addition, the next few stages will all 
+be finding ways to interpret the same bytecode at a lower and lower level, so keeping the bytecode 
+separate will make it clearer that it is not changed from stage to stage.\<close>
+
+text \<open>One unusual feature of the evaluation relation as we have written it is that the bytecode is 
+evaluated from right-to-left; that is, the operation at address x+1 will be executed before the 
+operation at x. This is mostly to simplify some later operations, in particular \<open>unflatten_code\<close>, 
+which relies on the code pointer always decreasing to prove termination.\<close>
+
+inductive eval\<^sub>b :: "code\<^sub>b list \<Rightarrow> state\<^sub>b \<Rightarrow> state\<^sub>b \<Rightarrow> bool" 
     (infix "\<tturnstile> _ \<leadsto>\<^sub>b" 50) where
-  evb_lookup [simp]: "lookup cd pc = Some (BLookup x) \<Longrightarrow> lookup env x = Some v \<Longrightarrow> 
-    cd \<tturnstile> BS vs ((env, Suc pc) # sfs) \<leadsto>\<^sub>b BS (v # vs) ((env, pc) # sfs)" 
-| evb_pushcon [simp]: "lookup cd pc = Some (BPushCon k) \<Longrightarrow> 
-    cd \<tturnstile> BS vs ((env, Suc pc) # sfs) \<leadsto>\<^sub>b BS (BConst k # vs) ((env, pc) # sfs)"
-| evb_pushlam [simp]: "lookup cd pc = Some (BPushLam pc') \<Longrightarrow> 
-    cd \<tturnstile> BS vs ((env, Suc pc) # sfs) \<leadsto>\<^sub>b BS (BLam env pc' # vs) ((env, pc) # sfs)"
-| evb_apply [simp]: "lookup cd pc = Some BApply \<Longrightarrow> 
-    cd \<tturnstile> BS (v # BLam env' pc' # vs) ((env, Suc pc) # sfs) \<leadsto>\<^sub>b 
-      BS vs ((v # env', pc') # (env, pc) # sfs)"
-| evb_return [simp]: "lookup cd pc = Some BReturn \<Longrightarrow> 
-    cd \<tturnstile> BS vs ((env, Suc pc) # sfs) \<leadsto>\<^sub>b BS vs sfs"
-| evb_jump [simp]: "lookup cd pc = Some BJump \<Longrightarrow> 
-    cd \<tturnstile> BS (v # BLam env' pc' # vs) ((env, Suc pc) # sfs) \<leadsto>\<^sub>b BS vs ((v # env', pc') # sfs)"
+  ev\<^sub>b_lookup [simp]: "lookup \<C> p = Some (Lookup\<^sub>b x) \<Longrightarrow> lookup \<Delta> x = Some v \<Longrightarrow> 
+    \<C> \<tturnstile> S\<^sub>b \<V> ((\<Delta>, Suc p) # s) \<leadsto>\<^sub>b S\<^sub>b (v # \<V>) ((\<Delta>, p) # s)" 
+| ev\<^sub>b_pushcon [simp]: "lookup \<C> p = Some (PushCon\<^sub>b n) \<Longrightarrow> 
+    \<C> \<tturnstile> S\<^sub>b \<V> ((\<Delta>, Suc p) # s) \<leadsto>\<^sub>b S\<^sub>b (Const\<^sub>b n # \<V>) ((\<Delta>, p) # s)"
+| ev\<^sub>b_pushlam [simp]: "lookup \<C> p = Some (PushLam\<^sub>b p') \<Longrightarrow> 
+    \<C> \<tturnstile> S\<^sub>b \<V> ((\<Delta>, Suc p) # s) \<leadsto>\<^sub>b S\<^sub>b (Lam\<^sub>b \<Delta> p' # \<V>) ((\<Delta>, p) # s)"
+| ev\<^sub>b_apply [simp]: "lookup \<C> p = Some Apply\<^sub>b \<Longrightarrow> 
+    \<C> \<tturnstile> S\<^sub>b (v # Lam\<^sub>b \<Delta>' p' # \<V>) ((\<Delta>, Suc p) # s) \<leadsto>\<^sub>b S\<^sub>b \<V> ((v # \<Delta>', p') # (\<Delta>, p) # s)"
+| ev\<^sub>b_return [simp]: "lookup \<C> p = Some Return\<^sub>b \<Longrightarrow> 
+    \<C> \<tturnstile> S\<^sub>b \<V> ((\<Delta>, Suc p) # s) \<leadsto>\<^sub>b S\<^sub>b \<V> s"
+| ev\<^sub>b_jump [simp]: "lookup \<C> p = Some Jump\<^sub>b \<Longrightarrow> 
+    \<C> \<tturnstile> S\<^sub>b (v # Lam\<^sub>b \<Delta>' p' # \<V>) ((\<Delta>, Suc p) # s) \<leadsto>\<^sub>b S\<^sub>b \<V> ((v # \<Delta>', p') # s)"
 
-theorem determinismb: "cd \<tturnstile> \<Sigma> \<leadsto>\<^sub>b \<Sigma>' \<Longrightarrow> cd \<tturnstile> \<Sigma> \<leadsto>\<^sub>b \<Sigma>'' \<Longrightarrow> \<Sigma>' = \<Sigma>''"
-proof (induction cd \<Sigma> \<Sigma>' rule: evalb.induct)
-  case (evb_lookup cd pc x env v vs sfs)
-  from evb_lookup(3, 1, 2) show ?case 
-    by (induction cd "BS vs ((env, Suc pc) # sfs)" \<Sigma>'' rule: evalb.induct) simp_all 
+theorem determinismb: "\<C> \<tturnstile> \<Sigma> \<leadsto>\<^sub>b \<Sigma>' \<Longrightarrow> \<C> \<tturnstile> \<Sigma> \<leadsto>\<^sub>b \<Sigma>'' \<Longrightarrow> \<Sigma>' = \<Sigma>''"
+proof (induction \<C> \<Sigma> \<Sigma>' rule: eval\<^sub>b.induct)
+  case ev\<^sub>b_lookup
+  from ev\<^sub>b_lookup(3, 1, 2) show ?case by (induction rule: eval\<^sub>b.cases) simp_all 
 next
-  case (evb_pushcon cd pc k vs env sfs)
-  from evb_pushcon(2, 1) show ?case 
-    by (induction cd "BS vs ((env, Suc pc) # sfs)" \<Sigma>'' rule: evalb.induct) simp_all 
+  case ev\<^sub>b_pushcon
+  from ev\<^sub>b_pushcon(2, 1) show ?case by (induction rule: eval\<^sub>b.cases) simp_all 
 next
-  case (evb_pushlam cd pc pc' vs env sfs)
-  from evb_pushlam(2, 1) show ?case 
-    by (induction cd "BS vs ((env, Suc pc) # sfs)" \<Sigma>'' rule: evalb.induct) simp_all 
+  case ev\<^sub>b_pushlam
+  from ev\<^sub>b_pushlam(2, 1) show ?case by (induction rule: eval\<^sub>b.cases) simp_all 
 next
-  case (evb_apply cd pc v env' pc' vs env sfs)
-  from evb_apply(2, 1) show ?case 
-    by (induction cd "BS (v # BLam env' pc' # vs) ((env, Suc pc) # sfs)" \<Sigma>'' rule: evalb.induct) 
-       simp_all 
+  case ev\<^sub>b_apply
+  from ev\<^sub>b_apply(2, 1) show ?case by (induction rule: eval\<^sub>b.cases) simp_all 
 next
-  case (evb_return cd pc vs env sfs)
-  from evb_return(2, 1) show ?case 
-    by (induction cd "BS vs ((env, Suc pc) # sfs)" \<Sigma>'' rule: evalb.induct) simp_all 
+  case ev\<^sub>b_return
+  from ev\<^sub>b_return(2, 1) show ?case by (induction rule: eval\<^sub>b.cases) simp_all 
 next
-  case (evb_jump cd pc v env' pc' vs env sfs)
-  from evb_jump(2, 1) show ?case 
-    by (induction cd "BS (v # BLam env' pc' # vs) ((env, Suc pc) # sfs)" \<Sigma>'' rule: evalb.induct) 
-       simp_all 
+  case ev\<^sub>b_jump
+  from ev\<^sub>b_jump(2, 1) show ?case by (induction rule: eval\<^sub>b.cases) simp_all 
 qed
+
+text \<open>We also define a properly-terminated predicate, indicating that the code is still structured 
+in blocks.\<close>
+
+primrec properly_terminated\<^sub>b :: "code\<^sub>b list \<Rightarrow> bool" where
+  "properly_terminated\<^sub>b [] = False"
+| "properly_terminated\<^sub>b (op # \<C>) = (op = Return\<^sub>b \<or> op = Jump\<^sub>b)"
+
 
 end
