07ByteCode/CodeFlattening.thy
@@ -2,94 +2,98 @@ theory CodeFlattening
   imports ByteCode "../06TreeCode/TreeCode"
 begin
 
-fun flatten_code' :: "nat \<Rightarrow> code\<^sub>e list \<Rightarrow> byte_code list" where
-  "flatten_code' lib [] = []"
-| "flatten_code' lib (Lookup\<^sub>e x # cd) = flatten_code' lib cd @ [BLookup x]"
-| "flatten_code' lib (PushCon\<^sub>e k # cd) = flatten_code' lib cd @ [BPushCon k]"
-| "flatten_code' lib (PushLam\<^sub>e cd' # cd) = (
-    let clo = flatten_code' lib cd'
-    in clo @ flatten_code' (lib + length clo) cd @ [BPushLam (lib + length clo)])"
-| "flatten_code' lib (Apply\<^sub>e # cd) = flatten_code' lib cd @ [BApply]"
-| "flatten_code' lib (Return\<^sub>e # cd) = flatten_code' lib cd @ [BReturn]"
-| "flatten_code' lib (Jump\<^sub>e # cd) = flatten_code' lib cd @ [BJump]"
+subsection \<open>Code Flattening\<close>
 
-definition flatten_code :: "code\<^sub>e list \<Rightarrow> byte_code list" where
-  "flatten_code cd \<equiv> flatten_code' 0 cd"
+text \<open>Flattening code is mostly just a map from tree-code operations to bytecode ones; but whenever 
+we reach a nested codeblock, we pull it out and convert it first. As a result, all code-pointers in
+the flattened codeblock point towards lower addresses. The first argument is the first free address;
+each nested codeblock is put there and then the argument is updated to its new, further-along 
+position.\<close>
 
-fun unflatten_code :: "byte_code list \<Rightarrow> nat \<Rightarrow> code\<^sub>e list" where
-  "unflatten_code cd 0 = []"
-| "unflatten_code cd (Suc pc) = (case lookup cd pc of
-      Some (BLookup x) \<Rightarrow> Lookup\<^sub>e x # unflatten_code cd pc
-    | Some (BPushCon k) \<Rightarrow>  PushCon\<^sub>e k # unflatten_code cd pc
-    | Some (BPushLam pc') \<Rightarrow> (
-        if pc' \<le> pc then PushLam\<^sub>e (unflatten_code cd pc') # unflatten_code cd pc else undefined) 
-    | Some BApply \<Rightarrow> Apply\<^sub>e # unflatten_code cd pc
-    | Some BReturn \<Rightarrow> [Return\<^sub>e]
-    | Some BJump \<Rightarrow> [Jump\<^sub>e]
+fun flatten_code' :: "nat \<Rightarrow> code\<^sub>e list \<Rightarrow> code\<^sub>b list" where
+  "flatten_code' p [] = []"
+| "flatten_code' p (Lookup\<^sub>e x # \<C>) = flatten_code' p \<C> @ [Lookup\<^sub>b x]"
+| "flatten_code' p (PushCon\<^sub>e n # \<C>) = flatten_code' p \<C> @ [PushCon\<^sub>b n]"
+| "flatten_code' p (PushLam\<^sub>e \<C>' # \<C>) = (
+    let \<C>\<^sub>b' = flatten_code' p \<C>'
+    in \<C>\<^sub>b' @ flatten_code' (p + length \<C>\<^sub>b') \<C> @ [PushLam\<^sub>b (p + length \<C>\<^sub>b')])"
+| "flatten_code' p (Apply\<^sub>e # \<C>) = flatten_code' p \<C> @ [Apply\<^sub>b]"
+| "flatten_code' p (Return\<^sub>e # \<C>) = flatten_code' p \<C> @ [Return\<^sub>b]"
+| "flatten_code' p (Jump\<^sub>e # \<C>) = flatten_code' p \<C> @ [Jump\<^sub>b]"
+
+definition flatten_code :: "code\<^sub>e list \<Rightarrow> code\<^sub>b list" where
+  "flatten_code \<C> \<equiv> flatten_code' 0 \<C>"
+
+text \<open>One might think that, like previous compilation passes, we could simply map \<open>flatten_code\<close> up
+the levels of the state and produce a compiled state. Unfortunately, we cannot. Once evaluation 
+begins, the code stored in the tree-code stack could come from all over the codebase, and there is 
+no guarantee that \<open>flatten_code\<close> would assign the right internal addresses. The structure of the 
+code would be the same, of course, but rather than get bogged down in trying to define an 
+"alpha-equivalence for code pointers" we cut to the chase and define a code-unflattening function.\<close>
+
+fun unflatten_code :: "code\<^sub>b list \<Rightarrow> nat \<Rightarrow> code\<^sub>e list" where
+  "unflatten_code \<C> 0 = []"
+| "unflatten_code \<C> (Suc p) = (case lookup \<C> p of
+      Some (Lookup\<^sub>b x) \<Rightarrow> Lookup\<^sub>e x # unflatten_code \<C> p
+    | Some (PushCon\<^sub>b n) \<Rightarrow>  PushCon\<^sub>e n # unflatten_code \<C> p
+    | Some (PushLam\<^sub>b p') \<Rightarrow> (
+        if p' \<le> p then PushLam\<^sub>e (unflatten_code \<C> p') # unflatten_code \<C> p else undefined) 
+    | Some Apply\<^sub>b \<Rightarrow> Apply\<^sub>e # unflatten_code \<C> p
+    | Some Return\<^sub>b \<Rightarrow> [Return\<^sub>e]
+    | Some Jump\<^sub>b \<Rightarrow> [Jump\<^sub>e]
     | None \<Rightarrow> undefined)"
 
-primrec unflatten_closure :: "byte_code list \<Rightarrow> bclosure \<Rightarrow> closure\<^sub>e" where
-  "unflatten_closure cd (BConst k) = Const\<^sub>e k"
-| "unflatten_closure cd (BLam vs pc) = Lam\<^sub>e (map (unflatten_closure cd) vs) (unflatten_code cd pc)"
+primrec unflatten_closure :: "code\<^sub>b list \<Rightarrow> closure\<^sub>b \<Rightarrow> closure\<^sub>e" where
+  "unflatten_closure \<C> (Const\<^sub>b n) = Const\<^sub>e n"
+| "unflatten_closure \<C> (Lam\<^sub>b \<Delta> p) = Lam\<^sub>e (map (unflatten_closure \<C>) \<Delta>) (unflatten_code \<C> p)"
 
-abbreviation ufcs :: "byte_code list \<Rightarrow> bclosure list \<Rightarrow> closure\<^sub>e list" where
-  "ufcs cd vs \<equiv> map (unflatten_closure cd) vs"
+abbreviation unflatten_values :: "code\<^sub>b list \<Rightarrow> closure\<^sub>b list \<Rightarrow> closure\<^sub>e list" where
+  "unflatten_values \<C> \<V> \<equiv> map (unflatten_closure \<C>) \<V>"
 
-primrec ufsf :: "byte_code list \<Rightarrow> (bclosure list \<times> nat) \<Rightarrow> frame\<^sub>e" where
-  "ufsf cd (vs, pc) = (ufcs cd vs, unflatten_code cd pc)"
+primrec unflatten_frame :: "code\<^sub>b list \<Rightarrow> (closure\<^sub>b list \<times> nat) \<Rightarrow> frame\<^sub>e" where
+  "unflatten_frame \<C> (\<Delta>, p) = (unflatten_values \<C> \<Delta>, unflatten_code \<C> p)"
 
-abbreviation ufsfs :: "byte_code list \<Rightarrow> (bclosure list \<times> nat) list \<Rightarrow> frame\<^sub>e list" where
-  "ufsfs cd pcs \<equiv> map (ufsf cd) pcs"
+abbreviation unflatten_stack :: "code\<^sub>b list \<Rightarrow> (closure\<^sub>b list \<times> nat) list \<Rightarrow> frame\<^sub>e list" where
+  "unflatten_stack \<C> s \<equiv> map (unflatten_frame \<C>) s"
 
-primrec unflatten_state :: "byte_code list \<Rightarrow> byte_code_state \<Rightarrow> state\<^sub>e" where
-  "unflatten_state cd (BS vs sfs) = S\<^sub>e (ufcs cd vs) (ufsfs cd sfs)"
+primrec unflatten_state :: "code\<^sub>b list \<Rightarrow> state\<^sub>b \<Rightarrow> state\<^sub>e" where
+  "unflatten_state \<C> (S\<^sub>b \<V> s) = S\<^sub>e (unflatten_values \<C> \<V>) (unflatten_stack \<C> s)"
+
+text \<open>We have noted already that all the pointers in the codebase should go towards smaller 
+addresses. We now define some predicates to assert this formally:\<close>
+
+fun orderly_op :: "nat \<Rightarrow> code\<^sub>b \<Rightarrow> bool" where
+  "orderly_op n (PushLam\<^sub>b p) = (0 < p \<and> p \<le> n)"
+| "orderly_op n _ = True"
+
+primrec orderly_code :: "code\<^sub>b list \<Rightarrow> nat \<Rightarrow> bool" where
+  "orderly_code [] n = True"
+| "orderly_code (op # cd) n = (orderly_op n op \<and> orderly_code cd (Suc n))"
+
+primrec orderly_closure :: "nat \<Rightarrow> closure\<^sub>b \<Rightarrow> bool" where
+  "orderly_closure n (Const\<^sub>b m) = True"
+| "orderly_closure n (Lam\<^sub>b \<Delta> p) = (0 < p \<and> p \<le> n \<and> list_all (orderly_closure n) \<Delta>)"
+
+fun orderly_stack :: "(closure\<^sub>b list \<times> nat) list \<Rightarrow> nat \<Rightarrow> bool" where
+  "orderly_stack [] n = True"
+| "orderly_stack ((\<Delta>, 0) # s) n = False"
+| "orderly_stack ((\<Delta>, Suc p) # s) n = 
+    (p < n \<and> list_all (orderly_closure n) \<Delta> \<and> orderly_stack s n)"
+
+primrec orderly_state :: "code\<^sub>b list \<Rightarrow> state\<^sub>b \<Rightarrow> bool" where
+  "orderly_state cd (S\<^sub>b vs sfs) = (orderly_code cd 0 \<and> properly_terminated\<^sub>b cd \<and> 
+    orderly_stack sfs (length cd) \<and> list_all (orderly_closure (length cd)) vs)"
 
 primrec code_size :: "code\<^sub>e \<Rightarrow> nat"
     and code_list_size :: "code\<^sub>e list \<Rightarrow> nat" where
   "code_size (Lookup\<^sub>e x) = 1"
-| "code_size (PushCon\<^sub>e k) = 1"
-| "code_size (PushLam\<^sub>e cd) = Suc (code_list_size cd)"
+| "code_size (PushCon\<^sub>e n) = 1"
+| "code_size (PushLam\<^sub>e \<C>) = Suc (code_list_size \<C>)"
 | "code_size Apply\<^sub>e = 1"
 | "code_size Return\<^sub>e = 1"
 | "code_size Jump\<^sub>e = 1"
 | "code_list_size [] = 0"
-| "code_list_size (c # cd) = code_size c + code_list_size cd"
-
-fun ordered :: "byte_code \<Rightarrow> nat \<Rightarrow> bool" where
-  "ordered (BPushLam pc) n = (0 < pc \<and> pc \<le> n)"
-| "ordered _ n = True"
-
-primrec ordered_closure :: "bclosure \<Rightarrow> nat \<Rightarrow> bool" 
-    and ordered_closures :: "bclosure list \<Rightarrow> nat \<Rightarrow> bool" where
-  "ordered_closure (BConst k) n = True"
-| "ordered_closure (BLam vs pc) n = (0 < pc \<and> pc \<le> n \<and> ordered_closures vs n)"
-| "ordered_closures [] n = True"
-| "ordered_closures (v # vs) n = (ordered_closure v n \<and> ordered_closures vs n)"
-
-primrec orderly :: "byte_code list \<Rightarrow> nat \<Rightarrow> bool" where
-  "orderly [] n = True"
-| "orderly (op # cd) n = (ordered op n \<and> orderly cd (Suc n))"
-
-primrec return_terminated\<^sub>b :: "byte_code list \<Rightarrow> bool" where
-  "return_terminated\<^sub>b [] = False"
-| "return_terminated\<^sub>b (op # cd) = (op = BReturn \<or> op = BJump)"
-
-fun return_terminated\<^sub>e :: "code\<^sub>e list \<Rightarrow> bool" where
-  "return_terminated\<^sub>e [] = False"
-| "return_terminated\<^sub>e (PushLam\<^sub>e cd' # cd) = (return_terminated\<^sub>e cd' \<and> return_terminated\<^sub>e cd)"
-| "return_terminated\<^sub>e (Return\<^sub>e # cd) = (cd = [])"
-| "return_terminated\<^sub>e (Jump\<^sub>e # cd) = (cd = [])"
-| "return_terminated\<^sub>e (op # cd) = return_terminated\<^sub>e cd"
-
-fun orderly_stack :: "(bclosure list \<times> nat) list \<Rightarrow> nat \<Rightarrow> bool" where
-  "orderly_stack [] cd = True"
-| "orderly_stack ((env, 0) # sfs) cd = False"
-| "orderly_stack ((env, Suc pc) # sfs) cd = 
-    (pc < cd \<and> ordered_closures env cd \<and> orderly_stack sfs cd)"
-
-primrec orderly_state :: "byte_code list \<Rightarrow> byte_code_state \<Rightarrow> bool" where
-  "orderly_state cd (BS vs sfs) = (orderly cd 0 \<and> return_terminated\<^sub>b cd \<and> 
-    orderly_stack sfs (length cd) \<and> ordered_closures vs (length cd))"
+| "code_list_size (op # \<C>) = code_size op + code_list_size \<C>"
 
 lemma flatten_length [simp]: "length (flatten_code' lib cd) = code_list_size cd"
   by (induction lib cd rule: flatten_code'.induct) simp_all
@@ -109,33 +113,33 @@ lemma [simp]: "(flatten_code' lib cd = []) = (cd = [])"
 lemma [simp]: "(flatten_code cd = []) = (cd = [])"
   by (simp add: flatten_code_def)
 
-lemma [simp]: "cd \<noteq> [] \<Longrightarrow> return_terminated\<^sub>b (cd @ cd') = return_terminated\<^sub>b cd"
+lemma [simp]: "cd \<noteq> [] \<Longrightarrow> properly_terminated\<^sub>b (cd @ cd') = properly_terminated\<^sub>b cd"
   by (induction cd) simp_all
 
-lemma return_terminated_flatten' [simp]: "return_terminated\<^sub>e cd \<Longrightarrow> 
-    return_terminated\<^sub>b (flatten_code' lib cd @ cd')"
+lemma return_terminated_flatten' [simp]: "properly_terminated\<^sub>e cd \<Longrightarrow> 
+    properly_terminated\<^sub>b (flatten_code' lib cd @ cd')"
   by (induction lib cd arbitrary: cd' rule: flatten_code'.induct) (auto split: if_splits)
 
-lemma [simp]: "return_terminated\<^sub>e cd \<Longrightarrow> return_terminated\<^sub>b (flatten_code cd)"
+lemma [simp]: "properly_terminated\<^sub>e cd \<Longrightarrow> properly_terminated\<^sub>b (flatten_code cd)"
 proof (unfold flatten_code_def)
-  assume "return_terminated\<^sub>e cd"
-  hence "return_terminated\<^sub>b (flatten_code' 0 cd @ [])" by (metis return_terminated_flatten')
-  thus "return_terminated\<^sub>b (flatten_code' 0 cd)" by simp
+  assume "properly_terminated\<^sub>e cd"
+  hence "properly_terminated\<^sub>b (flatten_code' 0 cd @ [])" by (metis return_terminated_flatten')
+  thus "properly_terminated\<^sub>b (flatten_code' 0 cd)" by simp
 qed
 
-lemma [simp]: "ordered op x \<Longrightarrow> ordered op (Suc x)"
+lemma [simp]: "orderly_op x op \<Longrightarrow> orderly_op (Suc x) op"
   by (induction op) simp_all
 
-lemma [simp]: "ordered op (x + n) \<Longrightarrow> ordered op (x + (m + n))"
+lemma [simp]: "orderly_op (x + n) op \<Longrightarrow> orderly_op (x + (m + n)) op"
   by (induction op) simp_all
 
-lemma [simp]: "orderly (cd @ cd') n = (orderly cd n \<and> orderly cd' (length cd + n))"
+lemma [simp]: "orderly_code (cd @ cd') n = (orderly_code cd n \<and> orderly_code cd' (length cd + n))"
   by (induction cd arbitrary: n) simp_all
 
-lemma [simp]: "lib \<le> n \<Longrightarrow> return_terminated\<^sub>e cd \<Longrightarrow> orderly (flatten_code' lib cd) n"
+lemma [simp]: "lib \<le> n \<Longrightarrow> properly_terminated\<^sub>e cd \<Longrightarrow> orderly_code (flatten_code' lib cd) n"
   by (induction lib cd arbitrary: n rule: flatten_code'.induct) auto
 
-lemma [simp]: "return_terminated\<^sub>e cdr \<Longrightarrow> orderly (flatten_code cdr) 0"
+lemma [simp]: "properly_terminated\<^sub>e cdr \<Longrightarrow> orderly_code (flatten_code cdr) 0"
   by (simp add: flatten_code_def)
 
 lemma [simp]: "x > 0 \<Longrightarrow> orderly_stack [([], x)] x"
@@ -153,14 +157,14 @@ proof -
   thus ?thesis by simp
 qed
  
-lemma [simp]: "lookup vs x = Some v \<Longrightarrow> ordered_closures vs n \<Longrightarrow> ordered_closure v n"
-  by (induction vs x rule: lookup.induct) simp_all
+lemma [simp]: "lookup vs x = Some v \<Longrightarrow> list_all (orderly_closure n) vs \<Longrightarrow> orderly_closure n v"
+  by auto
 
-lemma pushlam_ordered [simp]: "lookup cd x = Some (BPushLam pc) \<Longrightarrow> orderly cd n \<Longrightarrow> 
+lemma pushlam_ordered [simp]: "lookup cd x = Some (PushLam\<^sub>b pc) \<Longrightarrow> orderly_code cd n \<Longrightarrow> 
     x < length cd \<Longrightarrow> 0 < pc \<and> pc \<le> length cd + n"
   by (induction cd x arbitrary: n rule: lookup.induct) fastforce+
 
-lemma [simp]: "lookup cd x = Some (BPushLam pc) \<Longrightarrow> orderly cd 0 \<Longrightarrow> x < length cd \<Longrightarrow> 
+lemma [simp]: "lookup cd x = Some (PushLam\<^sub>b pc) \<Longrightarrow> orderly_code cd 0 \<Longrightarrow> x < length cd \<Longrightarrow> 
     0 < pc \<and> pc \<le> length cd"
   using pushlam_ordered by fastforce
 
@@ -177,200 +181,200 @@ qed
 
 lemma unflatten_front [simp]: "pc \<le> length cd \<Longrightarrow> 
     unflatten_code (cd @ cd') pc = unflatten_code cd pc"
-  by (induction cd pc rule: unflatten_code.induct) (simp_all split: option.splits byte_code.splits) 
+  by (induction cd pc rule: unflatten_code.induct) (simp_all split: option.splits code\<^sub>b.splits) 
 
-lemma unflatten_flatten [simp]: "return_terminated\<^sub>e cd \<Longrightarrow> 
+lemma unflatten_flatten [simp]: "properly_terminated\<^sub>e cd \<Longrightarrow> 
   unflatten_code (lib @ flatten_code' (length lib) cd @ acc) (length lib + code_list_size cd) = cd"
 proof (induction "length lib" cd arbitrary: lib acc rule: flatten_code'.induct)
   case (4 cd' cd)
   let ?pc = "length lib + code_list_size cd'"
   let ?code' = "lib @ flatten_code' (length lib) cd' @ []"
-  let ?code = "?code' @ flatten_code' ?pc cd @ BPushLam ?pc # acc"
+  let ?code = "?code' @ flatten_code' ?pc cd @ PushLam\<^sub>b ?pc # acc"
   have X: "length lib + length (flatten_code' (length lib) cd') = length ?code'" by simp
-  from 4 have "return_terminated\<^sub>e cd" by simp
+  from 4 have "properly_terminated\<^sub>e cd" by simp
   with 4 X have "unflatten_code (?code' @ flatten_code' (length ?code') cd @
-    BPushLam (length lib + length (flatten_code' (length lib) cd')) # acc)
+    PushLam\<^sub>b (length lib + length (flatten_code' (length lib) cd')) # acc)
       (length ?code' + code_list_size cd) = cd" by blast
   hence "unflatten_code ?code (length lib + code_list_size cd' + code_list_size cd) = cd" by simp
   hence X: "unflatten_code ?code (length lib + (code_list_size cd' + code_list_size cd)) = cd" 
     by (metis add.assoc)
-  from 4 have "return_terminated\<^sub>e cd'" by simp
+  from 4 have "properly_terminated\<^sub>e cd'" by simp
   with 4 have "unflatten_code ?code' (length lib + code_list_size cd') = cd'" by blast
   moreover have "?pc \<le> length ?code'" by simp
   ultimately have Z: "unflatten_code ?code ?pc =  cd'" by (metis unflatten_front)
   with X Z show ?case by simp
 qed simp_all
 
-lemma [simp]: "return_terminated\<^sub>e cd \<Longrightarrow> unflatten_code (flatten_code cd) (code_list_size cd) = cd"
+lemma [simp]: "properly_terminated\<^sub>e cd \<Longrightarrow> unflatten_code (flatten_code cd) (code_list_size cd) = cd"
 proof -
-  assume "return_terminated\<^sub>e cd"
+  assume "properly_terminated\<^sub>e cd"
   hence "unflatten_code ([] @ flatten_code' (length []) cd @ []) 
     (length [] + code_list_size cd) = cd" by (metis unflatten_flatten list.size(3))
   thus ?thesis by (simp add: flatten_code_def)
 qed
 
-lemma orderly_lam [simp]: "lookup cd pc = Some (BPushLam pc') \<Longrightarrow> orderly cd n \<Longrightarrow> pc' \<le> pc + n"
+lemma orderly_lam [simp]: "lookup cd pc = Some (PushLam\<^sub>b pc') \<Longrightarrow> orderly_code cd n \<Longrightarrow> pc' \<le> pc + n"
   by (induction cd pc arbitrary: n rule: lookup.induct) fastforce+
 
-lemma [simp]: "lookup cd pc = Some (BPushLam pc') \<Longrightarrow> orderly cd 0 \<Longrightarrow> pc' \<le> pc"
+lemma [simp]: "lookup cd pc = Some (PushLam\<^sub>b pc') \<Longrightarrow> orderly_code cd 0 \<Longrightarrow> pc' \<le> pc"
   using orderly_lam by fastforce
 
 theorem completeb [simp]: "cd \<tturnstile> \<Sigma>\<^sub>b \<leadsto>\<^sub>b \<Sigma>\<^sub>b' \<Longrightarrow> orderly_state cd \<Sigma>\<^sub>b \<Longrightarrow> 
   iter (\<leadsto>\<^sub>e) (unflatten_state cd \<Sigma>\<^sub>b) (unflatten_state cd \<Sigma>\<^sub>b')"
-proof (induction \<Sigma>\<^sub>b \<Sigma>\<^sub>b' rule: evalb.induct)
-  case (evb_lookup cd pc x env v vs sfs)
-  hence "S\<^sub>e (ufcs cd vs) 
-    ((ufcs cd env, unflatten_code cd (Suc pc)) # ufsfs cd sfs) \<leadsto>\<^sub>e
-      S\<^sub>e (unflatten_closure cd v # ufcs cd vs)
-        ((ufcs cd env, unflatten_code cd pc) # ufsfs cd sfs)" by simp
+proof (induction \<Sigma>\<^sub>b \<Sigma>\<^sub>b' rule: eval\<^sub>b.induct)
+  case (ev\<^sub>b_lookup cd pc x env v vs sfs)
+  hence "S\<^sub>e (unflatten_values cd vs) 
+    ((unflatten_values cd env, unflatten_code cd (Suc pc)) # unflatten_stack cd sfs) \<leadsto>\<^sub>e
+      S\<^sub>e (unflatten_closure cd v # unflatten_values cd vs)
+        ((unflatten_values cd env, unflatten_code cd pc) # unflatten_stack cd sfs)" by simp
   thus ?case by simp
 next
-  case (evb_pushcon cd pc k vs env sfs)
-  hence "S\<^sub>e (ufcs cd vs) 
-    ((ufcs cd env, unflatten_code cd (Suc pc)) # ufsfs cd sfs) \<leadsto>\<^sub>e
-      S\<^sub>e (Const\<^sub>e k # ufcs cd vs) 
-        ((ufcs cd env, unflatten_code cd pc) # ufsfs cd sfs)" by simp
+  case (ev\<^sub>b_pushcon cd pc k vs env sfs)
+  hence "S\<^sub>e (unflatten_values cd vs) 
+    ((unflatten_values cd env, unflatten_code cd (Suc pc)) # unflatten_stack cd sfs) \<leadsto>\<^sub>e
+      S\<^sub>e (Const\<^sub>e k # unflatten_values cd vs) 
+        ((unflatten_values cd env, unflatten_code cd pc) # unflatten_stack cd sfs)" by simp
   thus ?case by simp
 next
-  case (evb_pushlam cd pc pc' vs env sfs)
+  case (ev\<^sub>b_pushlam cd pc pc' vs env sfs)
   moreover hence X: "pc' \<le> pc" by auto
-  moreover have "iter (\<leadsto>\<^sub>e) (S\<^sub>e (ufcs cd vs) ((ufcs cd env, 
+  moreover have "iter (\<leadsto>\<^sub>e) (S\<^sub>e (unflatten_values cd vs) ((unflatten_values cd env, 
     PushLam\<^sub>e (unflatten_code cd pc') # 
-      unflatten_code cd pc) # ufsfs cd sfs))
-        (S\<^sub>e (Lam\<^sub>e (ufcs cd env) (unflatten_code cd pc') # ufcs cd vs) 
-          ((ufcs cd env, unflatten_code cd pc) # ufsfs cd sfs))" 
+      unflatten_code cd pc) # unflatten_stack cd sfs))
+        (S\<^sub>e (Lam\<^sub>e (unflatten_values cd env) (unflatten_code cd pc') # unflatten_values cd vs) 
+          ((unflatten_values cd env, unflatten_code cd pc) # unflatten_stack cd sfs))" 
     by (metis ev\<^sub>e_pushlam iter_one)
   ultimately show ?case by simp
 next
-  case (evb_apply cd pc v env' pc' vs env sfs)
-  hence "S\<^sub>e (unflatten_closure cd v # Lam\<^sub>e (ufcs cd env') (unflatten_code cd pc') # ufcs cd vs) 
-      ((ufcs cd env, unflatten_code cd (Suc pc)) # ufsfs cd sfs) \<leadsto>\<^sub>e
-        S\<^sub>e (ufcs cd vs) ((unflatten_closure cd v # ufcs cd env', unflatten_code cd pc') # 
-          (ufcs cd env, unflatten_code cd pc) # 
-            ufsfs cd sfs)" by simp
+  case (ev\<^sub>b_apply cd pc v env' pc' vs env sfs)
+  hence "S\<^sub>e (unflatten_closure cd v # Lam\<^sub>e (unflatten_values cd env') (unflatten_code cd pc') # unflatten_values cd vs) 
+      ((unflatten_values cd env, unflatten_code cd (Suc pc)) # unflatten_stack cd sfs) \<leadsto>\<^sub>e
+        S\<^sub>e (unflatten_values cd vs) ((unflatten_closure cd v # unflatten_values cd env', unflatten_code cd pc') # 
+          (unflatten_values cd env, unflatten_code cd pc) # 
+            unflatten_stack cd sfs)" by simp
   thus ?case by simp
 next
-  case (evb_return cd pc vs env sfs)
-  moreover have "iter (\<leadsto>\<^sub>e) (S\<^sub>e (ufcs cd vs) ((ufcs cd env, [Return\<^sub>e]) # ufsfs cd sfs))
-    (S\<^sub>e (ufcs cd vs) (ufsfs cd sfs))" by (metis ev\<^sub>e_return iter_one)
+  case (ev\<^sub>b_return cd pc vs env sfs)
+  moreover have "iter (\<leadsto>\<^sub>e) (S\<^sub>e (unflatten_values cd vs) ((unflatten_values cd env, [Return\<^sub>e]) # unflatten_stack cd sfs))
+    (S\<^sub>e (unflatten_values cd vs) (unflatten_stack cd sfs))" by (metis ev\<^sub>e_return iter_one)
   ultimately show ?case by simp
 next
-  case (evb_jump cd pc v env' pc' vs env sfs)
-  have "S\<^sub>e (unflatten_closure cd v # Lam\<^sub>e (ufcs cd env') (unflatten_code cd pc') # ufcs cd vs) 
-    ((ufcs cd env, [Jump\<^sub>e]) # ufsfs cd sfs) \<leadsto>\<^sub>e S\<^sub>e (ufcs cd vs)
-        ((unflatten_closure cd v # ufcs cd env', unflatten_code cd pc') # 
-          ufsfs cd sfs)" by (metis ev\<^sub>e_jump)
-  with evb_jump have "S\<^sub>e (unflatten_closure cd v # 
-    Lam\<^sub>e (ufcs cd env') (unflatten_code cd pc') # ufcs cd vs)
-      ((ufcs cd env, unflatten_code cd (Suc pc)) # ufsfs cd sfs) \<leadsto>\<^sub>e
-        S\<^sub>e (ufcs cd vs) ((unflatten_closure cd v # ufcs cd env', unflatten_code cd pc') # ufsfs cd sfs)" by simp
+  case (ev\<^sub>b_jump cd pc v env' pc' vs env sfs)
+  have "S\<^sub>e (unflatten_closure cd v # Lam\<^sub>e (unflatten_values cd env') (unflatten_code cd pc') # unflatten_values cd vs) 
+    ((unflatten_values cd env, [Jump\<^sub>e]) # unflatten_stack cd sfs) \<leadsto>\<^sub>e S\<^sub>e (unflatten_values cd vs)
+        ((unflatten_closure cd v # unflatten_values cd env', unflatten_code cd pc') # 
+          unflatten_stack cd sfs)" by (metis ev\<^sub>e_jump)
+  with ev\<^sub>b_jump have "S\<^sub>e (unflatten_closure cd v # 
+    Lam\<^sub>e (unflatten_values cd env') (unflatten_code cd pc') # unflatten_values cd vs)
+      ((unflatten_values cd env, unflatten_code cd (Suc pc)) # unflatten_stack cd sfs) \<leadsto>\<^sub>e
+        S\<^sub>e (unflatten_values cd vs) ((unflatten_closure cd v # unflatten_values cd env', unflatten_code cd pc') # unflatten_stack cd sfs)" by simp
   hence "iter (\<leadsto>\<^sub>e) (S\<^sub>e (unflatten_closure cd v # 
-    Lam\<^sub>e (ufcs cd env') (unflatten_code cd pc') # ufcs cd vs)
-      ((ufcs cd env, unflatten_code cd (Suc pc)) # ufsfs cd sfs))
-        (S\<^sub>e (ufcs cd vs) ((unflatten_closure cd v # ufcs cd env', unflatten_code cd pc') # ufsfs cd sfs))" 
+    Lam\<^sub>e (unflatten_values cd env') (unflatten_code cd pc') # unflatten_values cd vs)
+      ((unflatten_values cd env, unflatten_code cd (Suc pc)) # unflatten_stack cd sfs))
+        (S\<^sub>e (unflatten_values cd vs) ((unflatten_closure cd v # unflatten_values cd env', unflatten_code cd pc') # unflatten_stack cd sfs))" 
     by (metis iter_one)
   thus ?case by simp
 qed
 
 lemma [simp]: "Lam\<^sub>e envt cdt = unflatten_closure cdb vb \<Longrightarrow> 
-  \<exists>envb pc. vb = BLam envb pc \<and> envt = ufcs cdb envb \<and> cdt = unflatten_code cdb pc"
+  \<exists>envb pc. vb = Lam\<^sub>b envb pc \<and> envt = unflatten_values cdb envb \<and> cdt = unflatten_code cdb pc"
   by (induction vb) simp_all
 
 lemma unfl_state [dest]: "S\<^sub>e vs sfs = unflatten_state cd \<Sigma>\<^sub>b \<Longrightarrow> \<exists>vsb sfsb. 
-    \<Sigma>\<^sub>b = BS vsb sfsb \<and> vs = ufcs cd vsb \<and> sfs = ufsfs cd sfsb"
+    \<Sigma>\<^sub>b = S\<^sub>b vsb sfsb \<and> vs = unflatten_values cd vsb \<and> sfs = unflatten_stack cd sfsb"
   by (induction \<Sigma>\<^sub>b) simp_all
 
-lemma [dest]: "Lookup\<^sub>e x # cdt = unflatten_code cdb (Suc pc) \<Longrightarrow> orderly cdb 0 \<Longrightarrow> 
-    pc < length cdb \<Longrightarrow> lookup cdb pc = Some (BLookup x) \<and> cdt = unflatten_code cdb pc"
-  by (simp split: option.splits byte_code.splits)
+lemma [dest]: "Lookup\<^sub>e x # cdt = unflatten_code cdb (Suc pc) \<Longrightarrow> orderly_code cdb 0 \<Longrightarrow> 
+    pc < length cdb \<Longrightarrow> lookup cdb pc = Some (Lookup\<^sub>b x) \<and> cdt = unflatten_code cdb pc"
+  by (simp split: option.splits code\<^sub>b.splits)
 
-lemma [dest]: "PushCon\<^sub>e k # cdt = unflatten_code cdb (Suc pc) \<Longrightarrow> orderly cdb 0 \<Longrightarrow> 
-    pc < length cdb \<Longrightarrow> lookup cdb pc = Some (BPushCon k) \<and> cdt = unflatten_code cdb pc"
-  by (simp split: option.splits byte_code.splits)
+lemma [dest]: "PushCon\<^sub>e k # cdt = unflatten_code cdb (Suc pc) \<Longrightarrow> orderly_code cdb 0 \<Longrightarrow> 
+    pc < length cdb \<Longrightarrow> lookup cdb pc = Some (PushCon\<^sub>b k) \<and> cdt = unflatten_code cdb pc"
+  by (simp split: option.splits code\<^sub>b.splits)
 
 lemma [dest]: "PushLam\<^sub>e cdt'' # cdt = unflatten_code cdb (Suc pc) \<Longrightarrow> 
-  orderly cdb 0 \<Longrightarrow> pc < length cdb \<Longrightarrow>  
-    \<exists>pc'. lookup cdb pc = Some (BPushLam pc') \<and> cdt = unflatten_code cdb pc \<and> 
+  orderly_code cdb 0 \<Longrightarrow> pc < length cdb \<Longrightarrow>  
+    \<exists>pc'. lookup cdb pc = Some (PushLam\<^sub>b pc') \<and> cdt = unflatten_code cdb pc \<and> 
       cdt'' = unflatten_code cdb pc'"
-  by (simp split: option.splits byte_code.splits)
+  by (simp split: option.splits code\<^sub>b.splits)
 
-lemma [dest]: "Apply\<^sub>e # cdt = unflatten_code cdb (Suc pc) \<Longrightarrow> orderly cdb 0 \<Longrightarrow> 
-    pc < length cdb \<Longrightarrow> lookup cdb pc = Some BApply \<and> cdt = unflatten_code cdb pc"
-  by (simp split: option.splits byte_code.splits)
+lemma [dest]: "Apply\<^sub>e # cdt = unflatten_code cdb (Suc pc) \<Longrightarrow> orderly_code cdb 0 \<Longrightarrow> 
+    pc < length cdb \<Longrightarrow> lookup cdb pc = Some Apply\<^sub>b \<and> cdt = unflatten_code cdb pc"
+  by (simp split: option.splits code\<^sub>b.splits)
 
 lemma [dest]: "Return\<^sub>e # cd = unflatten_code cdb (Suc pc) \<Longrightarrow> 
-    orderly cdb 0 \<Longrightarrow> pc < length cdb \<Longrightarrow> lookup cdb pc = Some BReturn \<and> cd = []"
-  by (simp split: option.splits byte_code.splits)
+    orderly_code cdb 0 \<Longrightarrow> pc < length cdb \<Longrightarrow> lookup cdb pc = Some Return\<^sub>b \<and> cd = []"
+  by (simp split: option.splits code\<^sub>b.splits)
 
 lemma [dest]: "Jump\<^sub>e # cd = unflatten_code cdb (Suc pc) \<Longrightarrow> 
-    orderly cdb 0 \<Longrightarrow> pc < length cdb \<Longrightarrow> lookup cdb pc = Some BJump \<and> cd = []"
-  by (simp split: option.splits byte_code.splits)
+    orderly_code cdb 0 \<Longrightarrow> pc < length cdb \<Longrightarrow> lookup cdb pc = Some Jump\<^sub>b \<and> cd = []"
+  by (simp split: option.splits code\<^sub>b.splits)
 
-lemma uf_to_lookup [dest]: "(envt, Lookup\<^sub>e x # cdt) # sfst = ufsfs cdb sfsb \<Longrightarrow> 
-  orderly cdb 0 \<Longrightarrow> orderly_stack sfsb (length cdb) \<Longrightarrow> \<exists>envb pc sfsb'. 
-    sfsb = (envb, Suc pc) # sfsb' \<and> envt = ufcs cdb envb \<and> lookup cdb pc = Some (BLookup x) \<and> 
-      cdt = unflatten_code cdb pc \<and> sfst = ufsfs cdb sfsb'"
+lemma uf_to_lookup [dest]: "(envt, Lookup\<^sub>e x # cdt) # sfst = unflatten_stack cdb sfsb \<Longrightarrow> 
+  orderly_code cdb 0 \<Longrightarrow> orderly_stack sfsb (length cdb) \<Longrightarrow> \<exists>envb pc sfsb'. 
+    sfsb = (envb, Suc pc) # sfsb' \<and> envt = unflatten_values cdb envb \<and> lookup cdb pc = Some (Lookup\<^sub>b x) \<and> 
+      cdt = unflatten_code cdb pc \<and> sfst = unflatten_stack cdb sfsb'"
 proof (induction sfsb "length cdb" rule: orderly_stack.induct)
   case (3 envb pc sfsb')
-  hence "Lookup\<^sub>e x # cdt = unflatten_code cdb (Suc pc) \<and> orderly cdb 0 \<and> pc < length cdb" by simp
-  hence "lookup cdb pc = Some (BLookup x) \<and> cdt = unflatten_code cdb pc" by blast
+  hence "Lookup\<^sub>e x # cdt = unflatten_code cdb (Suc pc) \<and> orderly_code cdb 0 \<and> pc < length cdb" by simp
+  hence "lookup cdb pc = Some (Lookup\<^sub>b x) \<and> cdt = unflatten_code cdb pc" by blast
   with 3 show ?case by simp
 qed simp_all
 
-lemma uf_to_pushcon [dest]: "(envt, PushCon\<^sub>e k # cdt) # sfst = ufsfs cdb sfsb \<Longrightarrow> 
-  orderly cdb 0 \<Longrightarrow> orderly_stack sfsb (length cdb) \<Longrightarrow> 
-    \<exists>envb pc sfsb'. sfsb = (envb, Suc pc) # sfsb' \<and> envt = ufcs cdb envb \<and> 
-      lookup cdb pc = Some (BPushCon k) \<and> cdt = unflatten_code cdb pc \<and> sfst = ufsfs cdb sfsb'"
+lemma uf_to_pushcon [dest]: "(envt, PushCon\<^sub>e k # cdt) # sfst = unflatten_stack cdb sfsb \<Longrightarrow> 
+  orderly_code cdb 0 \<Longrightarrow> orderly_stack sfsb (length cdb) \<Longrightarrow> 
+    \<exists>envb pc sfsb'. sfsb = (envb, Suc pc) # sfsb' \<and> envt = unflatten_values cdb envb \<and> 
+      lookup cdb pc = Some (PushCon\<^sub>b k) \<and> cdt = unflatten_code cdb pc \<and> sfst = unflatten_stack cdb sfsb'"
 proof (induction sfsb "length cdb" rule: orderly_stack.induct)
   case (3 envb pc sfsb')
-  hence "PushCon\<^sub>e k # cdt = unflatten_code cdb (Suc pc) \<and> orderly cdb 0 \<and> pc < length cdb" by simp
-  hence "lookup cdb pc = Some (BPushCon k) \<and> cdt = unflatten_code cdb pc" by blast
+  hence "PushCon\<^sub>e k # cdt = unflatten_code cdb (Suc pc) \<and> orderly_code cdb 0 \<and> pc < length cdb" by simp
+  hence "lookup cdb pc = Some (PushCon\<^sub>b k) \<and> cdt = unflatten_code cdb pc" by blast
   with 3 show ?case by simp
 qed simp_all
 
-lemma uf_to_pushlam [dest]: "(envt, PushLam\<^sub>e cdt' # cdt) # sfst = ufsfs cdb sfsb \<Longrightarrow> 
-  orderly cdb 0 \<Longrightarrow> orderly_stack sfsb (length cdb) \<Longrightarrow> \<exists>envb pc sfsb' pc'. 
-    sfsb = (envb, Suc pc) # sfsb' \<and> envt = ufcs cdb envb \<and> lookup cdb pc = Some (BPushLam pc') \<and> 
-      cdt = unflatten_code cdb pc \<and> cdt' = unflatten_code cdb pc' \<and> sfst = ufsfs cdb sfsb'"
+lemma uf_to_pushlam [dest]: "(envt, PushLam\<^sub>e cdt' # cdt) # sfst = unflatten_stack cdb sfsb \<Longrightarrow> 
+  orderly_code cdb 0 \<Longrightarrow> orderly_stack sfsb (length cdb) \<Longrightarrow> \<exists>envb pc sfsb' pc'. 
+    sfsb = (envb, Suc pc) # sfsb' \<and> envt = unflatten_values cdb envb \<and> lookup cdb pc = Some (PushLam\<^sub>b pc') \<and> 
+      cdt = unflatten_code cdb pc \<and> cdt' = unflatten_code cdb pc' \<and> sfst = unflatten_stack cdb sfsb'"
 proof (induction sfsb "length cdb" rule: orderly_stack.induct)
   case (3 envb pc sfsb')
-  hence "PushLam\<^sub>e cdt' # cdt = unflatten_code cdb (Suc pc) \<and> orderly cdb 0 \<and> pc < length cdb" 
+  hence "PushLam\<^sub>e cdt' # cdt = unflatten_code cdb (Suc pc) \<and> orderly_code cdb 0 \<and> pc < length cdb" 
     by simp
-  then obtain pc' where "lookup cdb pc = Some (BPushLam pc') \<and> cdt = unflatten_code cdb pc \<and> 
+  then obtain pc' where "lookup cdb pc = Some (PushLam\<^sub>b pc') \<and> cdt = unflatten_code cdb pc \<and> 
     cdt' = unflatten_code cdb pc'" by blast
   with 3 show ?case by simp
 qed simp_all
 
-lemma uf_to_apply [dest]: "(envt, Apply\<^sub>e # cdt) # sfst = ufsfs cdb sfsb \<Longrightarrow> orderly cdb 0 \<Longrightarrow> 
+lemma uf_to_apply [dest]: "(envt, Apply\<^sub>e # cdt) # sfst = unflatten_stack cdb sfsb \<Longrightarrow> orderly_code cdb 0 \<Longrightarrow> 
   orderly_stack sfsb (length cdb) \<Longrightarrow> \<exists>envb pc sfsb'. sfsb = (envb, Suc pc) # sfsb' \<and> 
-    envt = ufcs cdb envb \<and> lookup cdb pc = Some BApply \<and> cdt = unflatten_code cdb pc \<and> 
-      sfst = ufsfs cdb sfsb'"
+    envt = unflatten_values cdb envb \<and> lookup cdb pc = Some Apply\<^sub>b \<and> cdt = unflatten_code cdb pc \<and> 
+      sfst = unflatten_stack cdb sfsb'"
 proof (induction sfsb "length cdb" rule: orderly_stack.induct)
   case (3 envb pc sfsb')
-  hence "Apply\<^sub>e # cdt = unflatten_code cdb (Suc pc) \<and> orderly cdb 0 \<and> pc < length cdb" by simp
-  hence "lookup cdb pc = Some BApply \<and> cdt = unflatten_code cdb pc" by blast
+  hence "Apply\<^sub>e # cdt = unflatten_code cdb (Suc pc) \<and> orderly_code cdb 0 \<and> pc < length cdb" by simp
+  hence "lookup cdb pc = Some Apply\<^sub>b \<and> cdt = unflatten_code cdb pc" by blast
   with 3 show ?case by simp
 qed simp_all
 
-lemma uf_to_return [dest]: "(envt, Return\<^sub>e # cd) # sfst = ufsfs cdb sfsb \<Longrightarrow> orderly cdb 0 \<Longrightarrow> 
+lemma uf_to_return [dest]: "(envt, Return\<^sub>e # cd) # sfst = unflatten_stack cdb sfsb \<Longrightarrow> orderly_code cdb 0 \<Longrightarrow> 
   orderly_stack sfsb (length cdb) \<Longrightarrow> \<exists>envb pc sfsb'. sfsb = (envb, Suc pc) # sfsb' \<and> 
-    envt = ufcs cdb envb \<and> lookup cdb pc = Some BReturn \<and> sfst = ufsfs cdb sfsb' \<and> cd = []"
+    envt = unflatten_values cdb envb \<and> lookup cdb pc = Some Return\<^sub>b \<and> sfst = unflatten_stack cdb sfsb' \<and> cd = []"
 proof (induction sfsb "length cdb" rule: orderly_stack.induct)
   case (3 envb pc sfsb')
   hence "Return\<^sub>e # cd = unflatten_code cdb (Suc pc) \<and> 
-    orderly cdb 0 \<and> pc < length cdb" by simp
-  hence "lookup cdb pc = Some BReturn \<and> cd = []" by blast
+    orderly_code cdb 0 \<and> pc < length cdb" by simp
+  hence "lookup cdb pc = Some Return\<^sub>b \<and> cd = []" by blast
   with 3 show ?case by simp
 qed simp_all
 
-lemma uf_to_jump [dest]: "(envt, Jump\<^sub>e # cd) # sfst = ufsfs cdb sfsb \<Longrightarrow> orderly cdb 0 \<Longrightarrow> 
+lemma uf_to_jump [dest]: "(envt, Jump\<^sub>e # cd) # sfst = unflatten_stack cdb sfsb \<Longrightarrow> orderly_code cdb 0 \<Longrightarrow> 
   orderly_stack sfsb (length cdb) \<Longrightarrow> \<exists>envb pc sfsb'. sfsb = (envb, Suc pc) # sfsb' \<and> 
-    envt = ufcs cdb envb \<and> lookup cdb pc = Some BJump \<and> sfst = ufsfs cdb sfsb'"
+    envt = unflatten_values cdb envb \<and> lookup cdb pc = Some Jump\<^sub>b \<and> sfst = unflatten_stack cdb sfsb'"
 proof (induction sfsb "length cdb" rule: orderly_stack.induct)
   case (3 envb pc sfsb')
   hence "Jump\<^sub>e # cd = unflatten_code cdb (Suc pc) \<and> 
-    orderly cdb 0 \<and> pc < length cdb" by simp
-  hence "lookup cdb pc = Some BJump \<and> cd = []" by blast
+    orderly_code cdb 0 \<and> pc < length cdb" by simp
+  hence "lookup cdb pc = Some Jump\<^sub>b \<and> cd = []" by blast
   with 3 show ?case by simp
 qed simp_all
 
@@ -378,111 +382,111 @@ theorem correctb [simp]: "unflatten_state cd\<^sub>b \<Sigma>\<^sub>b \<leadsto>
   \<exists>\<Sigma>\<^sub>b'. iter (\<tturnstile> cd\<^sub>b \<leadsto>\<^sub>b) \<Sigma>\<^sub>b \<Sigma>\<^sub>b' \<and> unflatten_state cd\<^sub>b \<Sigma>\<^sub>b' = \<Sigma>\<^sub>t'"
 proof (induction "unflatten_state cd\<^sub>b \<Sigma>\<^sub>b" \<Sigma>\<^sub>t' rule: eval\<^sub>e.induct)
   case (ev\<^sub>e_lookup env x v vs cd sfs)
-  then obtain vsb sfsb where B: "\<Sigma>\<^sub>b = BS vsb sfsb \<and> vs = ufcs cd\<^sub>b vsb \<and> 
-    (env, Lookup\<^sub>e x # cd) # sfs = ufsfs cd\<^sub>b sfsb" by fastforce
-  with ev\<^sub>e_lookup have "orderly cd\<^sub>b 0 \<and> orderly_stack sfsb (length cd\<^sub>b)" by simp
+  then obtain vsb sfsb where B: "\<Sigma>\<^sub>b = S\<^sub>b vsb sfsb \<and> vs = unflatten_values cd\<^sub>b vsb \<and> 
+    (env, Lookup\<^sub>e x # cd) # sfs = unflatten_stack cd\<^sub>b sfsb" by fastforce
+  with ev\<^sub>e_lookup have "orderly_code cd\<^sub>b 0 \<and> orderly_stack sfsb (length cd\<^sub>b)" by simp
   with B obtain envb pc sfsb' where S: "sfsb = (envb, Suc pc) # sfsb' \<and> 
-    env = ufcs cd\<^sub>b envb \<and> lookup cd\<^sub>b pc = Some (BLookup x) \<and> cd = unflatten_code cd\<^sub>b pc \<and> 
-      sfs = ufsfs cd\<^sub>b sfsb'" by (metis uf_to_lookup)
+    env = unflatten_values cd\<^sub>b envb \<and> lookup cd\<^sub>b pc = Some (Lookup\<^sub>b x) \<and> cd = unflatten_code cd\<^sub>b pc \<and> 
+      sfs = unflatten_stack cd\<^sub>b sfsb'" by (metis uf_to_lookup)
   with ev\<^sub>e_lookup obtain v' where V: "lookup envb x = Some v' \<and> unflatten_closure cd\<^sub>b v' = v"
     by fastforce
-  with S have "cd\<^sub>b \<tturnstile> BS vsb ((envb, Suc pc) # sfsb') \<leadsto>\<^sub>b BS (v' # vsb) ((envb, pc) # sfsb')"
+  with S have "cd\<^sub>b \<tturnstile> S\<^sub>b vsb ((envb, Suc pc) # sfsb') \<leadsto>\<^sub>b S\<^sub>b (v' # vsb) ((envb, pc) # sfsb')"
     by simp
-  hence "iter (\<tturnstile> cd\<^sub>b \<leadsto>\<^sub>b) (BS vsb ((envb, Suc pc) # sfsb')) (BS (v' # vsb) ((envb, pc) # sfsb'))" 
+  hence "iter (\<tturnstile> cd\<^sub>b \<leadsto>\<^sub>b) (S\<^sub>b vsb ((envb, Suc pc) # sfsb')) (S\<^sub>b (v' # vsb) ((envb, pc) # sfsb'))" 
     by simp
   with B S V show ?case by fastforce
 next
   case (ev\<^sub>e_pushcon vs env k cd sfs)
-  then obtain vsb sfsb where B: "\<Sigma>\<^sub>b = BS vsb sfsb \<and> vs = ufcs cd\<^sub>b vsb \<and> 
-    (env, PushCon\<^sub>e k # cd) # sfs = ufsfs cd\<^sub>b sfsb" by fastforce
-  with ev\<^sub>e_pushcon have "orderly cd\<^sub>b 0 \<and> orderly_stack sfsb (length cd\<^sub>b)" by simp
+  then obtain vsb sfsb where B: "\<Sigma>\<^sub>b = S\<^sub>b vsb sfsb \<and> vs = unflatten_values cd\<^sub>b vsb \<and> 
+    (env, PushCon\<^sub>e k # cd) # sfs = unflatten_stack cd\<^sub>b sfsb" by fastforce
+  with ev\<^sub>e_pushcon have "orderly_code cd\<^sub>b 0 \<and> orderly_stack sfsb (length cd\<^sub>b)" by simp
   with B obtain envb pc sfsb' where S: "sfsb = (envb, Suc pc) # sfsb' \<and> 
-    env = ufcs cd\<^sub>b envb \<and> lookup cd\<^sub>b pc = Some (BPushCon k) \<and> cd = unflatten_code cd\<^sub>b pc \<and> 
-      sfs = ufsfs cd\<^sub>b sfsb'" by (metis uf_to_pushcon)
-  with S have "cd\<^sub>b \<tturnstile> BS vsb ((envb, Suc pc) # sfsb') \<leadsto>\<^sub>b BS (BConst k # vsb) ((envb, pc) # sfsb')"
+    env = unflatten_values cd\<^sub>b envb \<and> lookup cd\<^sub>b pc = Some (PushCon\<^sub>b k) \<and> cd = unflatten_code cd\<^sub>b pc \<and> 
+      sfs = unflatten_stack cd\<^sub>b sfsb'" by (metis uf_to_pushcon)
+  with S have "cd\<^sub>b \<tturnstile> S\<^sub>b vsb ((envb, Suc pc) # sfsb') \<leadsto>\<^sub>b S\<^sub>b (Const\<^sub>b k # vsb) ((envb, pc) # sfsb')"
     by simp
-  hence "iter (\<tturnstile> cd\<^sub>b \<leadsto>\<^sub>b) (BS vsb ((envb, Suc pc) # sfsb')) 
-    (BS (BConst k # vsb) ((envb, pc) # sfsb'))" by simp
+  hence "iter (\<tturnstile> cd\<^sub>b \<leadsto>\<^sub>b) (S\<^sub>b vsb ((envb, Suc pc) # sfsb')) 
+    (S\<^sub>b (Const\<^sub>b k # vsb) ((envb, pc) # sfsb'))" by simp
   with B S show ?case by fastforce
 next
   case (ev\<^sub>e_pushlam vs env cd' cd sfs)
-  then obtain vsb sfsb where B: "\<Sigma>\<^sub>b = BS vsb sfsb \<and> vs = ufcs cd\<^sub>b vsb \<and> 
-    (env, PushLam\<^sub>e cd' # cd) # sfs = ufsfs cd\<^sub>b sfsb" by fastforce
-  with ev\<^sub>e_pushlam have "orderly cd\<^sub>b 0 \<and> orderly_stack sfsb (length cd\<^sub>b)" by simp
+  then obtain vsb sfsb where B: "\<Sigma>\<^sub>b = S\<^sub>b vsb sfsb \<and> vs = unflatten_values cd\<^sub>b vsb \<and> 
+    (env, PushLam\<^sub>e cd' # cd) # sfs = unflatten_stack cd\<^sub>b sfsb" by fastforce
+  with ev\<^sub>e_pushlam have "orderly_code cd\<^sub>b 0 \<and> orderly_stack sfsb (length cd\<^sub>b)" by simp
   with B obtain envb pc sfsb' pc' where S: "sfsb = (envb, Suc pc) # sfsb' \<and> 
-    env = ufcs cd\<^sub>b envb \<and> lookup cd\<^sub>b pc = Some (BPushLam pc') \<and> cd = unflatten_code cd\<^sub>b pc \<and> 
-      sfs = ufsfs cd\<^sub>b sfsb' \<and> cd' = unflatten_code cd\<^sub>b pc'" by (metis uf_to_pushlam)
-  with S have "cd\<^sub>b \<tturnstile> BS vsb ((envb, Suc pc) # sfsb') \<leadsto>\<^sub>b 
-    BS (BLam envb pc' # vsb) ((envb, pc) # sfsb')" by simp
-  hence "iter (\<tturnstile> cd\<^sub>b \<leadsto>\<^sub>b) (BS vsb ((envb, Suc pc) # sfsb')) 
-    (BS (BLam envb pc' # vsb) ((envb, pc) # sfsb'))" by simp
+    env = unflatten_values cd\<^sub>b envb \<and> lookup cd\<^sub>b pc = Some (PushLam\<^sub>b pc') \<and> cd = unflatten_code cd\<^sub>b pc \<and> 
+      sfs = unflatten_stack cd\<^sub>b sfsb' \<and> cd' = unflatten_code cd\<^sub>b pc'" by (metis uf_to_pushlam)
+  with S have "cd\<^sub>b \<tturnstile> S\<^sub>b vsb ((envb, Suc pc) # sfsb') \<leadsto>\<^sub>b 
+    S\<^sub>b (Lam\<^sub>b envb pc' # vsb) ((envb, pc) # sfsb')" by simp
+  hence "iter (\<tturnstile> cd\<^sub>b \<leadsto>\<^sub>b) (S\<^sub>b vsb ((envb, Suc pc) # sfsb')) 
+    (S\<^sub>b (Lam\<^sub>b envb pc' # vsb) ((envb, pc) # sfsb'))" by simp
   with B S show ?case by fastforce
 next
   case (ev\<^sub>e_apply v env' cd' vs env cd sfs)
-  then obtain vsb sfsb where B: "\<Sigma>\<^sub>b = BS vsb sfsb \<and> 
-    v # Lam\<^sub>e env' cd' # vs = ufcs cd\<^sub>b vsb \<and> (env, Apply\<^sub>e # cd) # sfs = ufsfs cd\<^sub>b sfsb" 
+  then obtain vsb sfsb where B: "\<Sigma>\<^sub>b = S\<^sub>b vsb sfsb \<and> 
+    v # Lam\<^sub>e env' cd' # vs = unflatten_values cd\<^sub>b vsb \<and> (env, Apply\<^sub>e # cd) # sfs = unflatten_stack cd\<^sub>b sfsb" 
       by fastforce
-  with ev\<^sub>e_apply have "orderly cd\<^sub>b 0 \<and> orderly_stack sfsb (length cd\<^sub>b)" by simp
+  with ev\<^sub>e_apply have "orderly_code cd\<^sub>b 0 \<and> orderly_stack sfsb (length cd\<^sub>b)" by simp
   with B obtain envb pc sfsb' where S: "sfsb = (envb, Suc pc) # sfsb' \<and> 
-    env = ufcs cd\<^sub>b envb \<and> lookup cd\<^sub>b pc = Some BApply \<and> cd = unflatten_code cd\<^sub>b pc \<and> 
-      sfs = ufsfs cd\<^sub>b sfsb'" by (metis uf_to_apply)
-  from B obtain vb envb' pc' vsb' where V: "vsb = vb # BLam envb' pc' # vsb' \<and> 
-    v = unflatten_closure cd\<^sub>b vb \<and> env' = ufcs cd\<^sub>b envb' \<and> cd' = unflatten_code cd\<^sub>b pc' \<and>
-      vs = ufcs cd\<^sub>b vsb'" by fastforce
-  from S have "cd\<^sub>b \<tturnstile> BS (vb # BLam envb' pc' # vsb') ((envb, Suc pc) # sfsb') \<leadsto>\<^sub>b
-    BS vsb' ((vb # envb', pc') # (envb, pc) # sfsb')" by simp
-  hence "iter (\<tturnstile> cd\<^sub>b \<leadsto>\<^sub>b) (BS (vb # BLam envb' pc' # vsb') ((envb, Suc pc) # sfsb')) 
-    (BS vsb' ((vb # envb', pc') # (envb, pc) # sfsb'))" by simp
+    env = unflatten_values cd\<^sub>b envb \<and> lookup cd\<^sub>b pc = Some Apply\<^sub>b \<and> cd = unflatten_code cd\<^sub>b pc \<and> 
+      sfs = unflatten_stack cd\<^sub>b sfsb'" by (metis uf_to_apply)
+  from B obtain vb envb' pc' vsb' where V: "vsb = vb # Lam\<^sub>b envb' pc' # vsb' \<and> 
+    v = unflatten_closure cd\<^sub>b vb \<and> env' = unflatten_values cd\<^sub>b envb' \<and> cd' = unflatten_code cd\<^sub>b pc' \<and>
+      vs = unflatten_values cd\<^sub>b vsb'" by fastforce
+  from S have "cd\<^sub>b \<tturnstile> S\<^sub>b (vb # Lam\<^sub>b envb' pc' # vsb') ((envb, Suc pc) # sfsb') \<leadsto>\<^sub>b
+    S\<^sub>b vsb' ((vb # envb', pc') # (envb, pc) # sfsb')" by simp
+  hence "iter (\<tturnstile> cd\<^sub>b \<leadsto>\<^sub>b) (S\<^sub>b (vb # Lam\<^sub>b envb' pc' # vsb') ((envb, Suc pc) # sfsb')) 
+    (S\<^sub>b vsb' ((vb # envb', pc') # (envb, pc) # sfsb'))" by simp
   with B S V show ?case by auto                                              
 next
   case (ev\<^sub>e_return vs env cd sfs)
-  then obtain vsb sfsb where B: "\<Sigma>\<^sub>b = BS vsb sfsb \<and> vs = ufcs cd\<^sub>b vsb \<and> 
-    (env, Return\<^sub>e # cd) # sfs = ufsfs cd\<^sub>b sfsb" by fastforce
-  with ev\<^sub>e_return have "orderly cd\<^sub>b 0 \<and> orderly_stack sfsb (length cd\<^sub>b)" by simp
+  then obtain vsb sfsb where B: "\<Sigma>\<^sub>b = S\<^sub>b vsb sfsb \<and> vs = unflatten_values cd\<^sub>b vsb \<and> 
+    (env, Return\<^sub>e # cd) # sfs = unflatten_stack cd\<^sub>b sfsb" by fastforce
+  with ev\<^sub>e_return have "orderly_code cd\<^sub>b 0 \<and> orderly_stack sfsb (length cd\<^sub>b)" by simp
   with B obtain envb pc sfsb' where S: "sfsb = (envb, Suc pc) # sfsb' \<and> 
-    env = ufcs cd\<^sub>b envb \<and> lookup cd\<^sub>b pc = Some BReturn \<and> sfs = ufsfs cd\<^sub>b sfsb'" 
+    env = unflatten_values cd\<^sub>b envb \<and> lookup cd\<^sub>b pc = Some Return\<^sub>b \<and> sfs = unflatten_stack cd\<^sub>b sfsb'" 
       by (metis uf_to_return)
-  with S have "cd\<^sub>b \<tturnstile> BS vsb ((envb, Suc pc) # sfsb') \<leadsto>\<^sub>b BS vsb sfsb'" by simp
-  hence "iter (\<tturnstile> cd\<^sub>b \<leadsto>\<^sub>b) (BS vsb ((envb, Suc pc) # sfsb')) (BS vsb sfsb')" by simp
+  with S have "cd\<^sub>b \<tturnstile> S\<^sub>b vsb ((envb, Suc pc) # sfsb') \<leadsto>\<^sub>b S\<^sub>b vsb sfsb'" by simp
+  hence "iter (\<tturnstile> cd\<^sub>b \<leadsto>\<^sub>b) (S\<^sub>b vsb ((envb, Suc pc) # sfsb')) (S\<^sub>b vsb sfsb')" by simp
   with B S show ?case by fastforce
 next
   case (ev\<^sub>e_jump v env' cd' vs env cd sfs)
-  then obtain vsb sfsb where B: "\<Sigma>\<^sub>b = BS vsb sfsb \<and> 
-    v # Lam\<^sub>e env' cd' # vs = ufcs cd\<^sub>b vsb \<and> 
-      (env, Jump\<^sub>e # cd) # sfs = ufsfs cd\<^sub>b sfsb" by fastforce
-  with ev\<^sub>e_jump have "orderly cd\<^sub>b 0 \<and> orderly_stack sfsb (length cd\<^sub>b)" by simp
+  then obtain vsb sfsb where B: "\<Sigma>\<^sub>b = S\<^sub>b vsb sfsb \<and> 
+    v # Lam\<^sub>e env' cd' # vs = unflatten_values cd\<^sub>b vsb \<and> 
+      (env, Jump\<^sub>e # cd) # sfs = unflatten_stack cd\<^sub>b sfsb" by fastforce
+  with ev\<^sub>e_jump have "orderly_code cd\<^sub>b 0 \<and> orderly_stack sfsb (length cd\<^sub>b)" by simp
   with B obtain envb pc sfsb' where S: "sfsb = (envb, Suc pc) # sfsb' \<and> 
-    env = ufcs cd\<^sub>b envb \<and> lookup cd\<^sub>b pc = Some BJump \<and> sfs = ufsfs cd\<^sub>b sfsb'" 
+    env = unflatten_values cd\<^sub>b envb \<and> lookup cd\<^sub>b pc = Some Jump\<^sub>b \<and> sfs = unflatten_stack cd\<^sub>b sfsb'" 
       by (metis uf_to_jump)
-  from B obtain vb envb' pc' vsb' where V: "vsb = vb # BLam envb' pc' # vsb' \<and> 
-    v = unflatten_closure cd\<^sub>b vb \<and> env' = ufcs cd\<^sub>b envb' \<and> cd' = unflatten_code cd\<^sub>b pc' \<and>
-      vs = ufcs cd\<^sub>b vsb'" by fastforce
-  from S have "cd\<^sub>b \<tturnstile> BS (vb # BLam envb' pc' # vsb') ((envb, Suc pc) # sfsb') \<leadsto>\<^sub>b
-    BS vsb' ((vb # envb', pc') # sfsb')" by simp
-  hence "iter (\<tturnstile> cd\<^sub>b \<leadsto>\<^sub>b) (BS (vb # BLam envb' pc' # vsb') ((envb, Suc pc) # sfsb')) 
-    (BS vsb' ((vb # envb', pc') # sfsb'))" by simp
+  from B obtain vb envb' pc' vsb' where V: "vsb = vb # Lam\<^sub>b envb' pc' # vsb' \<and> 
+    v = unflatten_closure cd\<^sub>b vb \<and> env' = unflatten_values cd\<^sub>b envb' \<and> cd' = unflatten_code cd\<^sub>b pc' \<and>
+      vs = unflatten_values cd\<^sub>b vsb'" by fastforce
+  from S have "cd\<^sub>b \<tturnstile> S\<^sub>b (vb # Lam\<^sub>b envb' pc' # vsb') ((envb, Suc pc) # sfsb') \<leadsto>\<^sub>b
+    S\<^sub>b vsb' ((vb # envb', pc') # sfsb')" by simp
+  hence "iter (\<tturnstile> cd\<^sub>b \<leadsto>\<^sub>b) (S\<^sub>b (vb # Lam\<^sub>b envb' pc' # vsb') ((envb, Suc pc) # sfsb')) 
+    (S\<^sub>b vsb' ((vb # envb', pc') # sfsb'))" by simp
   with B S V show ?case by auto                                              
 qed
 
 lemma [simp]: "cd\<^sub>b \<tturnstile> \<Sigma>\<^sub>b \<leadsto>\<^sub>b \<Sigma>\<^sub>b' \<Longrightarrow> orderly_state cd\<^sub>b \<Sigma>\<^sub>b \<Longrightarrow> orderly_state cd\<^sub>b \<Sigma>\<^sub>b'"
-proof (induction cd\<^sub>b \<Sigma>\<^sub>b \<Sigma>\<^sub>b' rule: evalb.induct)
-  case (evb_lookup cd pc x env v vs sfs)
+proof (induction cd\<^sub>b \<Sigma>\<^sub>b \<Sigma>\<^sub>b' rule: eval\<^sub>b.induct)
+  case (ev\<^sub>b_lookup cd pc x env v vs sfs)
   thus ?case by (cases pc, cases cd) simp_all
 next
-  case (evb_pushcon cd pc k vs env sfs)
+  case (ev\<^sub>b_pushcon cd pc k vs env sfs)
   thus ?case by (cases pc, cases cd) simp_all
 next
-  case (evb_pushlam cd pc pc' vs env sfs)
+  case (ev\<^sub>b_pushlam cd pc pc' vs env sfs)
   thus ?case 
   proof (cases pc)
     case 0
-    with evb_pushlam show ?thesis by (cases cd) simp_all
+    with ev\<^sub>b_pushlam show ?thesis by (cases cd) simp_all
   qed simp_all
 next
-  case (evb_apply cd pc v env' pc' vs env sfs)
+  case (ev\<^sub>b_apply cd pc v env' pc' vs env sfs)
   thus ?case by (cases pc', simp, cases pc, cases cd) simp_all
 next
-  case (evb_jump cd pc v env' pc' vs env sfs)
+  case (ev\<^sub>b_jump cd pc v env' pc' vs env sfs)
   thus ?case by (cases pc') simp_all
 qed simp_all
 
@@ -502,10 +506,10 @@ proof (induction "unflatten_state cd\<^sub>b \<Sigma>\<^sub>b" \<Sigma>\<^sub>t'
 qed force+
 
 lemma unfl_terminal [simp]: "unflatten_state cd \<Sigma> = S\<^sub>e [c] [] \<Longrightarrow>
-  \<exists>v. \<Sigma> = BS [v] [] \<and> c = unflatten_closure cd v"
+  \<exists>v. \<Sigma> = S\<^sub>b [v] [] \<and> c = unflatten_closure cd v"
 proof -
   assume "unflatten_state cd \<Sigma> = S\<^sub>e [c] []"
-  then obtain vs sfs where S: "\<Sigma> = BS vs sfs \<and> [c] = ufcs cd vs \<and> [] = ufsfs cd sfs" 
+  then obtain vs sfs where S: "\<Sigma> = S\<^sub>b vs sfs \<and> [c] = unflatten_values cd vs \<and> [] = unflatten_stack cd sfs" 
     by (metis unfl_state)
   moreover then obtain v where "vs = [v] \<and> c = unflatten_closure cd v" by blast
   ultimately show ?thesis by simp
@@ -513,14 +517,14 @@ qed
 
 lemma evalb_end [simp]: "iter (\<leadsto>\<^sub>e) (unflatten_state cd\<^sub>b \<Sigma>\<^sub>b) (S\<^sub>e [c] []) \<Longrightarrow> 
   orderly_state cd\<^sub>b \<Sigma>\<^sub>b \<Longrightarrow> 
-    \<exists>v. iter (\<tturnstile> cd\<^sub>b \<leadsto>\<^sub>b) \<Sigma>\<^sub>b (BS [v] []) \<and> c = unflatten_closure cd\<^sub>b v"
+    \<exists>v. iter (\<tturnstile> cd\<^sub>b \<leadsto>\<^sub>b) \<Sigma>\<^sub>b (S\<^sub>b [v] []) \<and> c = unflatten_closure cd\<^sub>b v"
 proof -
   assume "iter (\<leadsto>\<^sub>e) (unflatten_state cd\<^sub>b \<Sigma>\<^sub>b) (S\<^sub>e [c] [])"
   moreover assume O: "orderly_state cd\<^sub>b \<Sigma>\<^sub>b"
   ultimately obtain \<Sigma>\<^sub>b' where E: "iter (\<tturnstile> cd\<^sub>b \<leadsto>\<^sub>b) \<Sigma>\<^sub>b \<Sigma>\<^sub>b' \<and> unflatten_state cd\<^sub>b \<Sigma>\<^sub>b' = S\<^sub>e [c] []" 
     by fastforce
   moreover with O have "orderly_state cd\<^sub>b \<Sigma>\<^sub>b'" by fastforce
-  moreover with E obtain v where "\<Sigma>\<^sub>b' = BS [v] [] \<and> c = unflatten_closure cd\<^sub>b v" 
+  moreover with E obtain v where "\<Sigma>\<^sub>b' = S\<^sub>b [v] [] \<and> c = unflatten_closure cd\<^sub>b v" 
     by (metis unfl_terminal)
   ultimately show ?thesis by blast
 qed
