09ChainedEnvironment/ChainedEnvironment.thy
@@ -14,22 +14,22 @@ fun chain_lookup :: "('a \<times> ptr) heap \<Rightarrow> ptr \<Rightarrow> nat 
 | "chain_lookup h (Suc p) 0 = Some (case hlookup h p of (a, b) \<Rightarrow> a)"
 | "chain_lookup h (Suc p) (Suc x) = chain_lookup h (case hlookup h p of (a, b) \<Rightarrow> b) x"
 
-inductive evalce :: "byte_code list \<Rightarrow> chained_state \<Rightarrow> chained_state \<Rightarrow> bool" 
+inductive evalce :: "code\<^sub>b list \<Rightarrow> chained_state \<Rightarrow> chained_state \<Rightarrow> bool" 
     (infix "\<tturnstile> _ \<leadsto>\<^sub>c\<^sub>e" 50) where
-  evce_lookup [simp]: "lookup cd pc = Some (BLookup x) \<Longrightarrow> chain_lookup env p x = Some v \<Longrightarrow>
+  evce_lookup [simp]: "lookup cd pc = Some (Lookup\<^sub>b x) \<Longrightarrow> chain_lookup env p x = Some v \<Longrightarrow>
     cd \<tturnstile> CES h env vs ((p, Suc pc) # sfs) \<leadsto>\<^sub>c\<^sub>e CES h env (v # vs) ((p, pc) # sfs)"
-| evce_pushcon [simp]: "lookup cd pc = Some (BPushCon k) \<Longrightarrow> halloc h (CEConst k) = (h', v) \<Longrightarrow>
+| evce_pushcon [simp]: "lookup cd pc = Some (PushCon\<^sub>b k) \<Longrightarrow> halloc h (CEConst k) = (h', v) \<Longrightarrow>
     cd \<tturnstile> CES h env vs ((p, Suc pc) # sfs) \<leadsto>\<^sub>c\<^sub>e CES h' env (v # vs) ((p, pc) # sfs)"
-| evce_pushlam [simp]: "lookup cd pc = Some (BPushLam pc') \<Longrightarrow> 
+| evce_pushlam [simp]: "lookup cd pc = Some (PushLam\<^sub>b pc') \<Longrightarrow> 
     halloc h (CELam p pc') = (h', v) \<Longrightarrow> 
       cd \<tturnstile> CES h env vs ((p, Suc pc) # sfs) \<leadsto>\<^sub>c\<^sub>e CES h' env (v # vs) ((p, pc) # sfs)"
-| evce_apply [simp]: "lookup cd pc = Some BApply \<Longrightarrow> hlookup h v2 = CELam p' pc' \<Longrightarrow>
+| evce_apply [simp]: "lookup cd pc = Some Apply\<^sub>b \<Longrightarrow> hlookup h v2 = CELam p' pc' \<Longrightarrow>
     halloc env (v1, p') = (env', p'') \<Longrightarrow> 
       cd \<tturnstile> CES h env (v1 # v2 # vs) ((p, Suc pc) # sfs) \<leadsto>\<^sub>c\<^sub>e 
         CES h env' vs ((Suc p'', pc') # (p, pc) # sfs)"
-| evce_return [simp]: "lookup cd pc = Some BReturn \<Longrightarrow> 
+| evce_return [simp]: "lookup cd pc = Some Return\<^sub>b \<Longrightarrow> 
     cd \<tturnstile> CES h env vs ((p, Suc pc) # sfs) \<leadsto>\<^sub>c\<^sub>e CES h env vs sfs"
-| evce_jump [simp]: "lookup cd pc = Some BJump \<Longrightarrow> hlookup h v2 = CELam p' pc' \<Longrightarrow>
+| evce_jump [simp]: "lookup cd pc = Some Jump\<^sub>b \<Longrightarrow> hlookup h v2 = CELam p' pc' \<Longrightarrow>
     halloc env (v1, p') = (env', p'') \<Longrightarrow>
       cd \<tturnstile> CES h env (v1 # v2 # vs) ((p, Suc pc) # sfs) \<leadsto>\<^sub>c\<^sub>e CES h env' vs ((Suc p'', pc') # sfs)"
 
